merkel

Merkel.dfy
@@ -1,32 +1,127 @@
-// Machine ints for hashes.
-type uint32 = x: int | 0 <= x <= 0xFFFFFFFF
+// RUN: /compile:0  /rlimit:1000000
 
-// Assume there's some type for the data in the DAG.
-type Data
+module Prelude {
+    type Data
+    type Time = real
+    type uint32 = x: int | 0 <= x < 0xFFFFFFFF
+    type Hash = uint32
+    
+    function HashData(d: Data): Hash
+    function HashList(l: seq<Hash>): Hash
 
-// Assume there are some functions to manipulate hashes.
-function HashData(d: Data): uint32
-function HashCombine(n1: uint32, n2: uint32): uint32
-function HashSequence(s: seq<uint32>): uint32
-
-// Each node has some data, some children, and a hash summary.
-// The directedness of the structure is captured by the inductiveness
-// of this datatype: no node can have its ancestors as children.
-datatype MerkleNode = MerkleNode(data: Data, children: seq<MerkleNode>, hash: uint32)
-
-// Helper function to get a list of hashes from a list of nodes.
-function Hashes(l: seq<MerkleNode>): seq<uint32>
-{
-    if l == [] then
-        [] 
-    else 
-        [l[0].hash] + Hashes(l[1..])
+    function MapRemove<A(==),B>(m: map<A, B>, a: A): map<A, B>
+    {
+        map x | x in m && x != a :: m[x]
+    }
 }
 
-// What it means for a MerkleNode to be well formed: its children are
-// well formed, and its hash correctly summarizes the children and data.
-predicate MerkleNodeValid(m: MerkleNode)
-{
-    && (forall child | child in m.children :: MerkleNodeValid(child))
-    && m.hash == HashCombine(HashData(m.data), HashSequence(Hashes(m.children)))
+module Dedup {
+    import opened Prelude
+
+    datatype Dedup = 
+        | DChunk(data: Data, hash: Hash, KU: Time)
+        | DNode(children: seq<Hash>, hash: Hash, KU: Time)
+    
+    datatype State = State(dedups: map<Hash, Dedup>, refs: set<(Hash, Hash)>, now: Time)
+    
+    function DedupUpdateKU(d: Dedup, ku: Time): Dedup 
+    {
+        match d 
+            case DChunk(data, hash, _) => DChunk(data, hash, ku)
+            case DNode(children, hash, _) => DNode(children, hash, ku)
+    }
+
+    predicate DeleteDedup(s: State, s': State)
+    {
+        && s'.refs == s.refs
+        && s'.now == s.now
+        && exists hash {:trigger MapRemove(s.dedups, hash)} | hash in s.dedups :: 
+            var d := s.dedups[hash];
+            && d.KU < s.now
+            && (forall h | h in s.dedups && s.dedups[h].DNode? :: hash !in s.dedups[h].children)
+            && s'.dedups == MapRemove(s.dedups, hash)
+    }
+    
+    predicate ClockTick(s: State, s': State)
+    {
+        && s'.dedups == s.dedups
+        && s'.refs == s.refs
+        && s'.now >= s.now
+    }
+    
+    predicate ExtendKU(s: State, s': State, h: Hash, ku: Time)
+    {
+        && s'.refs == s.refs
+        && s'.now == s.now
+        && h in s.dedups
+        && var d := s.dedups[h];
+        && ku >= d.KU
+        && (d.DNode? ==> forall h' | h' in d.children && h' in s.dedups :: s.dedups[h'].KU >= ku)
+        && s'.dedups == s.dedups[h := DedupUpdateKU(d, ku)]
+    }
+
+    predicate Inv(s: State)
+    {
+        && (forall h, h' | h in s.dedups :: var d := s.dedups[h];
+            && d.DNode? 
+            && h' in d.children 
+            ==> 
+            && h' in s.dedups
+            && var d' := s.dedups[h'];
+            && d'.KU >= d.KU)
+    }
+
+    predicate Next(s: State, s': State)
+    {
+        || DeleteDedup(s, s')
+        || ClockTick(s, s')
+        || (exists h: Hash, ku :: ExtendKU(s, s', h, ku))
+    }
+
+    lemma InvInductive(s: State, s': State)
+        requires Inv(s) && Next(s, s')
+        ensures Inv(s')
+    { }
+}
+
+
+module DedupTree {
+    import opened Prelude
+    import Dedup
+
+    datatype DedupTree = 
+        | DTChunk(data: Data, hash: Hash, KU: Time)
+        | DTNode(children: seq<DedupTree>, hash: Hash, KU: Time)
+    
+    predicate InTree(d: Dedup.Dedup, t: DedupTree)
+    {
+        match t
+            case DTChunk(data, hash, KU) => d == Dedup.DChunk(data, hash, KU)
+            case DTNode(children, hash, KU) => 
+                || d == Dedup.DNode(Hashes(children), hash, KU)
+                || exists c | c in children :: InTree(d, c)
+    }
+    
+    function Hashes(l: seq<DedupTree>): seq<Hash>
+    {
+        if l == [] then
+            []
+        else 
+            [l[0].hash] + Hashes(l[1..])
+    }
+    
+    predicate DedupTreeValid(m: DedupTree)
+    {
+        match m 
+            case DTChunk(d,h,_) => h == HashData(d)
+            case DTNode(children, h, ku) => 
+                && (forall child | child in children :: DedupTreeValid(child) && ku <= child.KU)
+                && h == HashList(Hashes(children))
+    }
+    
+    predicate DedupsMatchTrees(dedups: map<Hash, Dedup.Dedup>, trees: set<DedupTree>)
+    {
+        && (forall h | h in dedups :: exists t | t in trees :: InTree(dedups[h], t))
+        && (forall t, d | t in trees && InTree(d, t) :: d.hash in dedups && dedups[d.hash] == d)
+    }
 }
